some more progress

examples/wysteria/examples/fstar_main/dealiface.fsi
@@ -10,4 +10,5 @@ open FStar.OrdSet
 
 type sh
 
-val deal: ps:prins{ps = union (union (singleton Alice) (singleton Bob)) (singleton Charlie)} -> p:prin{mem p ps} -> shares:list sh -> rands:int -> deal_to:prin -> Tot (list sh * int)
+val deal: ps:prins{ps = union (union (singleton Alice) (singleton Bob)) (singleton Charlie)} -> p:prin{mem p ps} -> shares:list sh -> rands:int -> deal_to:prin -> Tot int
+(* val deal: ps:prins{ps = union (union (singleton Alice) (singleton Bob)) (singleton Charlie)} -> p:prin{mem p ps} -> shares:list sh -> rands:int -> deal_to:prin -> Tot (list sh * int) *)
