examples/wysteria/examples/fstar_main/dealiface.ml
@@ -8,5 +8,5 @@ let deal ps p shares rands deal_to =
   let e2 = mk_const (C_opaque ((), Obj.magic shares, T_cons ("Prims.list", [ T_sh;]))) in
   let e3 = mk_mkwire (mk_const (C_eprins (singleton p))) (mk_box (mk_const (C_eprins (singleton p))) (mk_const (C_opaque ((), Obj.magic rands, T_cons ("Prims.int", []))))) in
   let e4 = mk_const (C_prin deal_to) in
-  let dv = Interpreteriface.run p "deal" T_unknown [e1; e2; e3; e4] in
+  let dv = Interpreteriface.run p "deal" T_unknown [e1; e2; e3; e4] false in
   Obj.magic (Interpreteriface.project_value_content dv)
