examples/wysteria/ml/interpreteriface.ml
@@ -26,14 +26,15 @@ let init_env =
     else if name_of_var x = "bob" then Some (D_v (const_meta, V_prin Bob))
     else if name_of_var x = "charlie" then Some (D_v (const_meta, V_prin Charlie))
     else None
-           
-let run (p:prin) (fn:string) (t:typ) (l:exp list) :dvalue =
+
+(* the boolean indicates whether to add mk_projwire, deal passes false *)
+let run (p:prin) (fn:string) (t:typ) (l:exp list) (b:bool) :dvalue =
   let e_main = mk_app (mk_var fn t) (List.hd l) in
   let e_main = List.fold_left (fun acc e -> mk_app acc e) e_main (List.tl l) in
   let e_c = List.fold_left (fun acc (x, t, e) ->
     mk_let (mk_varname x t) e acc
   ) e_main (List.rev program) in
-  let e = mk_projwire (mk_const (C_prin p)) e_c in
+  let e = if b then mk_projwire (mk_const (C_prin p)) e_c else e_c in
   let dv_opt = Interpreter.run p init_env e in
   match dv_opt with
     | None    -> raise Not_found
