examples/wysteria/examples/fstar_main/deal.fst
@@ -46,7 +46,8 @@ val deal:
   ps:prins{ps = abc}
   -> shares:list (Sh int){forall x. FStar.List.mem x shares ==> ps_of_sh x = abc}
   -> rands:Wire int ps -> deal_to:prin
-  -> Wys (list (Sh int) * int) (pre (Mode Par abc)) post
+//  -> Wys (list (Sh int) * int) (pre (Mode Par abc)) post
+  -> Wys int (pre (Mode Par abc)) post
 let deal ps shares rands deal_to =
   let proj: p:prin{FStar.OrdSet.mem p abc} -> unit
 	    -> Wys int (pre (Mode Par (singleton p))) post =
@@ -62,20 +63,29 @@ let deal ps shares rands deal_to =
     let r1' = unbox_s r1 in
     let r2' = unbox_s r2 in
     let r3' = unbox_s r3 in
-    let t1 = r1' + r2' in
-    let t2 = r3' + t1 in
-    mk_sh t2
+    let t1 = r1' > r2' in
+    let t2 = r3' = r1' in
+    mk_sh r1'
+    (* let t1 = r1' + r2' in *)
+    (* let t2 = r3' + t1 in *)
+    (* mk_sh t2 *)
   in
 
   let new_sh = as_sec abc add in
 
   let card: unit -> Wys int (pre (Mode Sec abc)) post =
-    fun _ -> comb_sh new_sh
+    fun _ ->
+    let r1' = unbox_s r1 in
+    let r2' = unbox_s r2 in
+    let r3' = unbox_s r3 in
+    let t1 = r1' > r2' in
+    let t2 = r3' = r1' in
+    comb_sh new_sh
   in
 
   let c = as_sec abc card in
-  
-  let fresh = check_fresh shares new_sh in
+  c
+  (* let fresh = check_fresh shares new_sh in *)
 
-  if fresh then mk_tuple (mk_cons new_sh shares) c
-  else mk_tuple shares c
+  (* if fresh then mk_tuple (mk_cons new_sh shares) c *)
+  (* else mk_tuple shares c *)
